

# Vector Operations

Neil Christian A. Sagun

September 3, 2023

**1. Let  $\mathbf{u} = (1, -2, 4)$ ,  $\mathbf{v} = (3, 5, 1)$ , and  $\mathbf{w} = (2, 1, -3)$ .**

**a.  $3\mathbf{u} - 2\mathbf{v}$**

The result of  $3\mathbf{u} - 2\mathbf{v}$  is:

$$\begin{aligned} 3\mathbf{u} - 2\mathbf{v} &= 3(1, -2, 4) - 2(3, 5, 1) \\ &= (3, -6, 12) - (6, 10, 2) \\ &= (-3, -16, 10) \end{aligned}$$

**b.  $5\mathbf{u} + 3\mathbf{v} - 4\mathbf{w}$**

The result of  $5\mathbf{u} + 3\mathbf{v} - 4\mathbf{w}$  is:

$$\begin{aligned} 5\mathbf{u} + 3\mathbf{v} - 4\mathbf{w} &= 5(1, -2, 4) + 3(3, 5, 1) - 4(2, 1, -3) \\ &= (5, -10, 20) + (9, 15, 3) - (8, 4, +12) \\ &= (6, 1, 35) \end{aligned}$$

**c.  $\mathbf{u} \cdot \mathbf{v}$ ,  $\mathbf{v} \cdot \mathbf{w}$ ,  $\mathbf{u} \cdot \mathbf{w}$**

The dot products are:

$$\begin{aligned} \mathbf{u} \cdot \mathbf{v} &= (1, -2, 4) \cdot (3, 5, 1) = (1)(3) + (-2)(5) + (4)(1) = 3 - 10 + 4 = -3 \\ \mathbf{v} \cdot \mathbf{w} &= (3, 5, 1) \cdot (2, 1, -3) = (3)(2) + (5)(1) + (1)(-3) = 6 + 5 - 3 = 8 \\ \mathbf{u} \cdot \mathbf{w} &= (1, -2, 4) \cdot (2, 1, -3) = (1)(2) + (-2)(1) + (4)(-3) = 2 - 2 - 12 = -12 \end{aligned}$$

**d.  $\|\mathbf{u}\|$ ,  $\|\mathbf{v}\|$ ,  $\|\mathbf{w}\|$**

The magnitudes are:

$$\begin{aligned} \|\mathbf{u}\| &= \sqrt{1^2 + (-2)^2 + 4^2} = \sqrt{1 + 4 + 16} = \sqrt{21} \\ \|\mathbf{v}\| &= \sqrt{3^2 + 5^2 + 1^2} = \sqrt{9 + 25 + 1} = \sqrt{35} \\ \|\mathbf{w}\| &= \sqrt{2^2 + 1^2 + (-3)^2} = \sqrt{4 + 1 + 9} = \sqrt{14} \end{aligned}$$

**e. If  $\theta$  is the angle between  $\mathbf{u}$  and  $\mathbf{v}$ , find  $\cos \theta$**

The cosine of the angle  $\theta$  between  $\mathbf{u}$  and  $\mathbf{v}$  can be calculated using the dot product and magnitudes:

$$\cos \theta = \frac{\mathbf{u} \cdot \mathbf{v}}{\|\mathbf{u}\|\|\mathbf{v}\|} = \frac{-3}{\sqrt{21}\sqrt{35}}$$

**f. If  $\theta$  is the angle between  $\mathbf{v}$  and  $\mathbf{w}$ , find  $\cos \theta$**

The cosine of the angle  $\theta$  between  $\mathbf{v}$  and  $\mathbf{w}$  can be calculated using the dot product and magnitudes:

$$\cos \theta = \frac{\mathbf{v} \cdot \mathbf{w}}{\|\mathbf{v}\| \|\mathbf{w}\|} = \frac{8}{\sqrt{35}\sqrt{14}}$$

**g. If  $\theta$  is the angle between  $\mathbf{u}$  and  $\mathbf{w}$ , find  $\cos \theta$**

The cosine of the angle  $\theta$  between  $\mathbf{u}$  and  $\mathbf{w}$  can be calculated using the dot product and magnitudes:

$$\cos \theta = \frac{\mathbf{u} \cdot \mathbf{w}}{\|\mathbf{u}\| \|\mathbf{w}\|} = \frac{-12}{\sqrt{21}\sqrt{14}}$$

**h. Find distance( $\mathbf{u}$ ,  $\mathbf{v}$ )**

The distance between  $\mathbf{u}$  and  $\mathbf{v}$  is:

$$\begin{aligned} \text{distance}(\mathbf{u}, \mathbf{v}) &= \|\mathbf{u} - \mathbf{v}\| \\ &= \|(1, -2, 4) - (3, 5, 1)\| \\ &= \|(-2, -7, 3)\| \\ &= \sqrt{(-2)^2 + (-7)^2 + 3^2} \\ &= \sqrt{4 + 49 + 9} \\ &= \sqrt{62} \end{aligned}$$

**i. Find distance( $\mathbf{w}$ ,  $\mathbf{v}$ )**

The distance between  $\mathbf{w}$  and  $\mathbf{v}$  is:

$$\begin{aligned} \text{distance}(\mathbf{w}, \mathbf{v}) &= \|\mathbf{w} - \mathbf{v}\| \\ &= \|(2, 1, -3) - (3, 5, 1)\| \\ &= \|(-1, -4, -4)\| \\ &= \sqrt{(-1)^2 + (-4)^2 + (-4)^2} \\ &= \sqrt{1 + 16 + 16} \\ &= \sqrt{33} \end{aligned}$$

**j. Find distance( $\mathbf{u}$ ,  $\mathbf{w}$ )**

The distance between  $\mathbf{u}$  and  $\mathbf{w}$  is:

$$\begin{aligned} \text{distance}(\mathbf{u}, \mathbf{w}) &= \|\mathbf{u} - \mathbf{w}\| \\ &= \|(1, -2, 4) - (2, 1, -3)\| \\ &= \|(-1, -3, 7)\| \\ &= \sqrt{(-1)^2 + (-3)^2 + 7^2} \\ &= \sqrt{1 + 9 + 49} \\ &= \sqrt{59} \end{aligned}$$

**k. Find  $\text{projection}(\mathbf{u}, \mathbf{v})$** 

The projection of  $\mathbf{v}$  onto  $\mathbf{u}$  is:

$$\begin{aligned}\text{projection}(\mathbf{u}, \mathbf{v}) &= \frac{\mathbf{u} \cdot \mathbf{v}}{\|\mathbf{v}\|^2} \mathbf{v} \\ &= \frac{-3}{35} (3, 5, 1) \\ &= \left(-\frac{9}{35}, -\frac{15}{35}, -\frac{3}{35}\right)\end{aligned}$$

**l. Find  $\text{projection}(\mathbf{w}, \mathbf{v})$** 

The projection of  $\mathbf{v}$  onto  $\mathbf{w}$  is:

$$\begin{aligned}\text{projection}(\mathbf{w}, \mathbf{v}) &= \frac{\mathbf{w} \cdot \mathbf{v}}{\|\mathbf{v}\|^2} \mathbf{v} \\ &= \frac{8}{35} (3, 5, 1) \\ &= \left(\frac{24}{35}, \frac{40}{35}, \frac{8}{35}\right)\end{aligned}$$

**m. Find  $\text{projection}(\mathbf{u}, \mathbf{w})$** 

The projection of  $\mathbf{w}$  onto  $\mathbf{u}$  is:

$$\begin{aligned}\text{projection}(\mathbf{u}, \mathbf{w}) &= \frac{\mathbf{u} \cdot \mathbf{w}}{\|\mathbf{w}\|^2} \mathbf{w} \\ &= \frac{-12}{14} (2, 1, -3) \\ &= \left(-\frac{12}{7}, -\frac{6}{7}, \frac{18}{7}\right)\end{aligned}$$

**2. Let  $\mathbf{u} = (1, 3, -4)$ ,  $\mathbf{v} = (2, 1, 5)$ , and  $\mathbf{w} = (3, -2, 6)$ .****a.  $3\mathbf{u} - 2\mathbf{v}$** 

The result of  $3\mathbf{u} - 2\mathbf{v}$  is:

$$\begin{aligned}3\mathbf{u} - 2\mathbf{v} &= 3 \begin{pmatrix} 1 \\ 3 \\ -4 \end{pmatrix} - 2 \begin{pmatrix} 2 \\ 1 \\ 5 \end{pmatrix} \\ &= \begin{pmatrix} 3 \\ 9 \\ -12 \end{pmatrix} - \begin{pmatrix} 4 \\ 2 \\ 10 \end{pmatrix} \\ &= \begin{pmatrix} -1 \\ 7 \\ -22 \end{pmatrix}\end{aligned}$$

**b.  $5\mathbf{u} + 3\mathbf{v} - 4\mathbf{w}$** 

The result of  $5\mathbf{u} + 3\mathbf{v} - 4\mathbf{w}$  is:

$$\begin{aligned}5\mathbf{u} + 3\mathbf{v} - 4\mathbf{w} &= 5 \begin{pmatrix} 1 \\ 3 \\ -4 \end{pmatrix} + 3 \begin{pmatrix} 2 \\ 1 \\ 5 \end{pmatrix} - 4 \begin{pmatrix} 3 \\ -2 \\ 6 \end{pmatrix} \\ &= \begin{pmatrix} 5 \\ 15 \\ -20 \end{pmatrix} + \begin{pmatrix} 6 \\ 3 \\ 15 \end{pmatrix} - \begin{pmatrix} 12 \\ +8 \\ 24 \end{pmatrix}\end{aligned}$$

$$= \begin{pmatrix} -1 \\ 26 \\ -29 \end{pmatrix}$$

**c.  $\mathbf{u} \cdot \mathbf{v}$ ,  $\mathbf{v} \cdot \mathbf{w}$ ,  $\mathbf{u} \cdot \mathbf{w}$**

The dot products are:

$$\mathbf{u} \cdot \mathbf{v} = \begin{pmatrix} 1 \\ 3 \\ -4 \end{pmatrix} \cdot \begin{pmatrix} 2 \\ 1 \\ 5 \end{pmatrix} = (1)(2) + (3)(1) + (-4)(5) = 2 + 3 - 20 = -15$$

$$\mathbf{v} \cdot \mathbf{w} = \begin{pmatrix} 2 \\ 1 \\ 5 \end{pmatrix} \cdot \begin{pmatrix} 3 \\ -2 \\ 6 \end{pmatrix} = (2)(3) + (1)(-2) + (5)(6) = 6 - 2 + 30 = 34$$

$$\mathbf{u} \cdot \mathbf{w} = \begin{pmatrix} 1 \\ 3 \\ -4 \end{pmatrix} \cdot \begin{pmatrix} 3 \\ -2 \\ 6 \end{pmatrix} = (1)(3) + (3)(-2) + (-4)(6) = 3 - 6 - 24 = -27$$

**d.  $\|\mathbf{u}\|$ ,  $\|\mathbf{v}\|$ ,  $\|\mathbf{w}\|$**

The magnitudes are:

$$\|\mathbf{u}\| = \sqrt{1^2 + 3^2 + (-4)^2} = \sqrt{1 + 9 + 16} = \sqrt{26}$$

$$\|\mathbf{v}\| = \sqrt{2^2 + 1^2 + 5^2} = \sqrt{4 + 1 + 25} = \sqrt{30}$$

$$\|\mathbf{w}\| = \sqrt{3^2 + (-2)^2 + 6^2} = \sqrt{9 + 4 + 36} = \sqrt{49} = 7$$

**e. If  $\theta$  is the angle between  $\mathbf{u}$  and  $\mathbf{v}$ , find  $\cos \theta$**

The cosine of the angle  $\theta$  between  $\mathbf{u}$  and  $\mathbf{v}$  can be calculated using the dot product and magnitudes:

$$\cos \theta = \frac{\mathbf{u} \cdot \mathbf{v}}{\|\mathbf{u}\| \|\mathbf{v}\|} = \frac{-15}{\sqrt{26}\sqrt{30}}$$

**f. If  $\theta$  is the angle between  $\mathbf{v}$  and  $\mathbf{w}$ , find  $\cos \theta$**

The cosine of the angle  $\theta$  between  $\mathbf{v}$  and  $\mathbf{w}$  can be calculated using the dot product and magnitudes:

$$\cos \theta = \frac{\mathbf{v} \cdot \mathbf{w}}{\|\mathbf{v}\| \|\mathbf{w}\|} = \frac{34}{\sqrt{30} \cdot 7}$$

**g. If  $\theta$  is the angle between  $\mathbf{u}$  and  $\mathbf{w}$ , find  $\cos \theta$**

The cosine of the angle  $\theta$  between  $\mathbf{u}$  and  $\mathbf{w}$  can be calculated using the dot product and magnitudes:

$$\cos \theta = \frac{\mathbf{u} \cdot \mathbf{w}}{\|\mathbf{u}\| \|\mathbf{w}\|} = \frac{-27}{\sqrt{26} \cdot 7}$$

**h. Find distance( $\mathbf{u}, \mathbf{v}$ )**

The distance between  $\mathbf{u}$  and  $\mathbf{v}$  is:

$$\begin{aligned} \text{distance}(\mathbf{u}, \mathbf{v}) &= \|\mathbf{u} - \mathbf{v}\| \\ &= \left\| \begin{pmatrix} 1 \\ 3 \\ -4 \end{pmatrix} - \begin{pmatrix} 2 \\ 1 \\ 5 \end{pmatrix} \right\| \end{aligned}$$

$$\begin{aligned}
&= \left\| \begin{pmatrix} -1 \\ 2 \\ -9 \end{pmatrix} \right\| \\
&= \sqrt{(-1)^2 + 2^2 + (-9)^2} \\
&= \sqrt{1 + 4 + 81} \\
&= \sqrt{86}
\end{aligned}$$

**i. Find distance(**w**, **v**)**

The distance between **w** and **v** is:

$$\begin{aligned}
\text{distance}(\mathbf{w}, \mathbf{v}) &= \|\mathbf{w} - \mathbf{v}\| \\
&= \left\| \begin{pmatrix} 3 \\ -2 \\ 6 \end{pmatrix} - \begin{pmatrix} 2 \\ 1 \\ 5 \end{pmatrix} \right\| \\
&= \left\| \begin{pmatrix} 1 \\ -3 \\ 1 \end{pmatrix} \right\| \\
&= \sqrt{1^2 + (-3)^2 + 1^2} \\
&= \sqrt{1 + 9 + 1} \\
&= \sqrt{11}
\end{aligned}$$

**j. Find distance(**u**, **w**)**

The distance between **u** and **w** is:

$$\begin{aligned}
\text{distance}(\mathbf{u}, \mathbf{w}) &= \|\mathbf{u} - \mathbf{w}\| \\
&= \left\| \begin{pmatrix} 1 \\ 3 \\ -4 \end{pmatrix} - \begin{pmatrix} 3 \\ -2 \\ 6 \end{pmatrix} \right\| \\
&= \left\| \begin{pmatrix} -2 \\ 5 \\ -10 \end{pmatrix} \right\| \\
&= \sqrt{(-2)^2 + 5^2 + (-10)^2} \\
&= \sqrt{4 + 25 + 100} \\
&= \sqrt{129}
\end{aligned}$$

**k. Find projection(**u**, **v**)**

The projection of **v** onto **u** is:

$$\begin{aligned}
\text{projection}(\mathbf{u}, \mathbf{v}) &= \frac{\mathbf{u} \cdot \mathbf{v}}{\|\mathbf{v}\|^2} \mathbf{v} \\
&= \frac{-15}{30} \begin{pmatrix} 2 \\ 1 \\ 5 \end{pmatrix} \\
&= -\frac{1}{2} \begin{pmatrix} 2 \\ 1 \\ 5 \end{pmatrix} \\
&= \begin{pmatrix} -\frac{1}{7} \\ \frac{2}{7} \\ -\frac{4}{7} \end{pmatrix}
\end{aligned}$$

### l. Find projection( $\mathbf{w}, \mathbf{v}$ )

The projection of  $\mathbf{v}$  onto  $\mathbf{w}$  is:

$$\begin{aligned}\text{projection}(\mathbf{w}, \mathbf{v}) &= \frac{\mathbf{w} \cdot \mathbf{v}}{\|\mathbf{v}\|^2} \mathbf{v} \\ &= \frac{34}{30} \begin{pmatrix} 2 \\ 1 \\ 5 \end{pmatrix} \\ &= \frac{17}{15} \begin{pmatrix} 2 \\ 1 \\ 5 \end{pmatrix} \\ &= \begin{pmatrix} \frac{34}{15} \\ \frac{17}{15} \\ \frac{85}{15} \end{pmatrix}\end{aligned}$$

### m. Find projection( $\mathbf{u}, \mathbf{w}$ )

The projection of  $\mathbf{w}$  onto  $\mathbf{u}$  is:

$$\begin{aligned}\text{projection}(\mathbf{u}, \mathbf{w}) &= \frac{\mathbf{u} \cdot \mathbf{w}}{\|\mathbf{w}\|^2} \mathbf{w} \\ &= \frac{-27}{49} \begin{pmatrix} 3 \\ -2 \\ 6 \end{pmatrix} \\ &= -\frac{27}{49} \begin{pmatrix} 3 \\ -2 \\ 6 \end{pmatrix} \\ &= \begin{pmatrix} -\frac{81}{49} \\ \frac{54}{49} \\ -\frac{162}{49} \end{pmatrix}\end{aligned}$$

### 3. Let $\mathbf{u} = (2, -5, 4, 6, -3)$ and $\mathbf{v} = (5, -2, 1, -7, -4)$ $\mathbf{w} = (2, 1, -3)$ find:

#### a. $4\mathbf{u} - 3\mathbf{v}$

The result of  $4\mathbf{u} - 3\mathbf{v}$  is:

$$4\mathbf{u} - 3\mathbf{v} = (8, -20, 16, 24, -12) - (15, -6, 3, -21, -12) = (-7, -14, 13, 45, 0).$$

#### b. $5\mathbf{u} + 2\mathbf{v} - 2\mathbf{w}$

The result of  $5\mathbf{u} + 2\mathbf{v} - 2\mathbf{w}$  is:

$$5\mathbf{u} + 2\mathbf{v} - 2\mathbf{w} = (10, -25, 20, 30, -15) + (10, -4, 2, -14, -8) - (4, 2, -6, 0, 0) = (16, -31, 28, 16, -23).$$

#### c. $\mathbf{u} \cdot \mathbf{v}$ , $\mathbf{v} \cdot \mathbf{w}$ , $\mathbf{u} \cdot \mathbf{w}$

The dot products are:

$$\mathbf{u} \cdot \mathbf{v} = (2)(5) + (-5)(-2) + (4)(1) + (6)(-7) + (-3)(-4) = 10 + 10 + 4 - 42 + 12 = -6$$

$$\mathbf{v} \cdot \mathbf{w} = (5)(2) + (-2)(1) + (1)(-3) + (-7)(0) + (-4)(0) = 10 - 2 - 3 + 0 + 0 = 5$$

$$\mathbf{u} \cdot \mathbf{w} = (2)(2) + (-5)(1) + (4)(-3) + (6)(0) + (-3)(0) = 4 - 5 - 12 + 0 + 0 = -13$$

**d.  $\|\mathbf{u}\|$ ,  $\|\mathbf{v}\|$ ,  $\|\mathbf{w}\|$**

The magnitudes are:

$$\|\mathbf{u}\| = \sqrt{2^2 + (-5)^2 + 4^2 + 6^2 + (-3)^2} = \sqrt{4 + 25 + 16 + 36 + 9} = \sqrt{90}$$

$$\|\mathbf{v}\| = \sqrt{5^2 + (-2)^2 + 1^2 + (-7)^2 + (-4)^2} = \sqrt{25 + 4 + 1 + 49 + 16} = \sqrt{95}$$

$$\|\mathbf{w}\| = \sqrt{2^2 + 1^2 + (-3)^2 + 0^2 + 0^2} = \sqrt{4 + 1 + 9 + 0 + 0} = \sqrt{14}$$

**e. If  $\theta$  is the angle between  $\mathbf{u}$  and  $\mathbf{v}$ , find  $\cos \theta$**

The cosine of the angle  $\theta$  between  $\mathbf{u}$  and  $\mathbf{v}$  can be calculated using the dot product and magnitudes:

$$\cos \theta = \frac{\mathbf{u} \cdot \mathbf{v}}{\|\mathbf{u}\| \|\mathbf{v}\|} = \frac{-6}{\sqrt{90}\sqrt{95}}$$

**f. If  $\theta$  is the angle between  $\mathbf{v}$  and  $\mathbf{w}$ , find  $\cos \theta$**

The cosine of the angle  $\theta$  between  $\mathbf{v}$  and  $\mathbf{w}$  can be calculated using the dot product and magnitudes:

$$\cos \theta = \frac{\mathbf{v} \cdot \mathbf{w}}{\|\mathbf{v}\| \|\mathbf{w}\|} = \frac{5}{\sqrt{95}\sqrt{14}}$$

**g. If  $\theta$  is the angle between  $\mathbf{u}$  and  $\mathbf{w}$ , find  $\cos \theta$**

The cosine of the angle  $\theta$  between  $\mathbf{u}$  and  $\mathbf{w}$  can be calculated using the dot product and magnitudes:

$$\cos \theta = \frac{\mathbf{u} \cdot \mathbf{w}}{\|\mathbf{u}\| \|\mathbf{w}\|} = \frac{-13}{\sqrt{90}\sqrt{14}}$$

**h. Find distance( $\mathbf{u}$ ,  $\mathbf{v}$ )**

The distance between  $\mathbf{u}$  and  $\mathbf{v}$  is:

$$\begin{aligned} \text{distance}(\mathbf{u}, \mathbf{v}) &= \|\mathbf{u} - \mathbf{v}\| = \|(2, -5, 4, 6, -3) - (5, -2, 1, -7, -4)\| \\ &= \|(-3, -3, 3, 13, 1)\| \\ &= \sqrt{(-3)^2 + (-3)^2 + 3^2 + 13^2 + 1^2} \\ &= \sqrt{9 + 9 + 9 + 169 + 1} \\ &= \sqrt{197} \end{aligned}$$

**i. Find distance( $\mathbf{w}$ ,  $\mathbf{v}$ )**

The distance between  $\mathbf{w}$  and  $\mathbf{v}$  is:

$$\begin{aligned} \text{distance}(\mathbf{w}, \mathbf{v}) &= \|\mathbf{w} - \mathbf{v}\| = \|(2, 1, -3, 0, 0) - (5, -2, 1, -7, -4)\| \\ &= \|(-3, 3, -4, 7, 4)\| \\ &= \sqrt{(-3)^2 + 3^2 + (-4)^2 + 7^2 + 4^2} \\ &= \sqrt{9 + 9 + 16 + 49 + 16} \\ &= \sqrt{99} \end{aligned}$$

**j. Find distance( $\mathbf{u}, \mathbf{w}$ )**

The distance between  $\mathbf{u}$  and  $\mathbf{w}$  is:

$$\begin{aligned}
 \text{distance}(\mathbf{u}, \mathbf{w}) &= \|\mathbf{u} - \mathbf{w}\| = \|(2, 1, -3, 0, 0) - (5, -2, 1, -7, -4)\| \\
 &= \|(0, -6, 7, 6, -3)\| \\
 &= \sqrt{0^2 + (-6)^2 + 7^2 + 6^2 + (-3)^2} \\
 &= \sqrt{0 + 36 + 49 + 36 + 9} \\
 &= \sqrt{130}
 \end{aligned}$$

**k. Find projection( $\mathbf{u}, \mathbf{v}$ )**

The projection of  $\mathbf{v}$  onto  $\mathbf{u}$  is:

$$\begin{aligned}
 \text{projection}(\mathbf{u}, \mathbf{v}) &= \frac{\mathbf{u} \cdot \mathbf{v}}{\|\mathbf{v}\|^2} \mathbf{v} \\
 &= \frac{-6}{\|\mathbf{v}\|^2} (5, -2, 1, -7, -4) \\
 &= \frac{-6}{(\sqrt{95})^2} (5, -2, 1, -7, -4) \\
 &= \frac{-6}{95} (5, -2, 1, -7, -4) \\
 &= \left( -\frac{30}{95}, \frac{12}{95}, -\frac{6}{95}, \frac{42}{95}, \frac{24}{95} \right).
 \end{aligned}$$

**l. Find projection( $\mathbf{w}, \mathbf{v}$ )**

The projection of  $\mathbf{v}$  onto  $\mathbf{w}$  is:

$$\begin{aligned}
 \text{projection}(\mathbf{w}, \mathbf{v}) &= \frac{\mathbf{w} \cdot \mathbf{v}}{\|\mathbf{v}\|^2} \mathbf{v} \\
 &= \frac{5}{\|\mathbf{v}\|^2} (5, -2, 1, -7, -4) \\
 &= \frac{5}{(\sqrt{95})^2} (5, -2, 1, -7, -4) \\
 &= \frac{5}{95} (5, -2, 1, -7, -4) \\
 &= \left( \frac{25}{95}, -\frac{10}{95}, -\frac{5}{95}, -\frac{35}{95}, -\frac{20}{95} \right).
 \end{aligned}$$

**m. Find projection( $\mathbf{u}, \mathbf{w}$ )**

The projection of  $\mathbf{w}$  onto  $\mathbf{u}$  is:

$$\begin{aligned}
 \text{projection}(\mathbf{u}, \mathbf{w}) &= \frac{\mathbf{u} \cdot \mathbf{w}}{\|\mathbf{w}\|^2} \mathbf{w} \\
 &= \frac{-13}{\|\mathbf{w}\|^2} (2, 1, -3, 0, 0) \\
 &= \frac{-13}{(\sqrt{14})^2} (2, 1, -3, 0, 0) \\
 &= \frac{-13}{14} (2, 1, -3, 0, 0) \\
 &= \left( -\frac{26}{95}, -\frac{13}{95}, \frac{26}{95}, 0, 0 \right).
 \end{aligned}$$



#### 4. Normalize each vector:

##### a. Normalized vector $\mathbf{u}$ :

$$\|\mathbf{u}\| = \sqrt{5^2 + (-7)^2} = \sqrt{74}$$
$$\hat{\mathbf{u}} = \frac{\mathbf{u}}{\|\mathbf{u}\|} = \left( \frac{5}{\sqrt{74}}, -\frac{7}{\sqrt{74}} \right).$$

##### b. Normalized vector $\mathbf{v}$ :

$$\|\mathbf{v}\| = \sqrt{1^2 + 2^2 + (-2)^2 + 4^2} = 5$$
$$\hat{\mathbf{v}} = \frac{\mathbf{v}}{\|\mathbf{v}\|} = \left( \frac{1}{5}, \frac{2}{5}, -\frac{2}{5}, \frac{4}{5} \right).$$

##### c. Normalized vector $\mathbf{w}$ :

$$\|\mathbf{w}\| = \left[ \frac{1}{2}, -\frac{1}{3}, \frac{3}{4} \right] \left( \frac{1}{2} \cdot \frac{1}{2} \right) + \left( -\frac{1}{3} \cdot -\frac{1}{3} \right) + \left( \frac{3}{4} \cdot \frac{3}{4} \right)$$
$$\|\mathbf{w}\| = \frac{1}{4} + \frac{1}{9} + \frac{9}{16}$$
$$\|\mathbf{w}\| = \frac{29}{16}$$
$$\|\mathbf{w}\| = \sqrt{w \cdot w} = \sqrt{\frac{29}{16}}$$
$$\hat{\mathbf{w}} = \frac{\mathbf{w}}{\|\mathbf{w}\|} = \left( \frac{1}{\sqrt{\frac{29}{16}}}, -\frac{1}{\sqrt{\frac{29}{16}}}, \frac{3}{\sqrt{\frac{29}{16}}} \right).$$

#### 5. Let $\mathbf{u} = (1, 2, -2)$ , $\mathbf{v} = (3, -12, 4)$ and a scalar $k = -3$

##### a. The norm (magnitude) of vector $\mathbf{u}$ , denoted as $\|\mathbf{u}\|$ , is given by:

$$\|\mathbf{u}\| = \sqrt{1^2 + 2^2 + (-2)^2} = \sqrt{1 + 4 + 4} = \sqrt{9} = 3$$

So,  $\|\mathbf{u}\| = 3$ .

##### b. The norm (magnitude) of vector $\mathbf{v}$ , denoted as $\|\mathbf{v}\|$ , is given by:

$$\|\mathbf{v}\| = \sqrt{3^2 + (-12)^2 + 4^2} = \sqrt{9 + 144 + 16} = \sqrt{169} = 13$$

So,  $\|\mathbf{v}\| = 13$ .

##### c. The norm (magnitude) of the vector sum $\mathbf{u} + \mathbf{v}$ , denoted as $\|\mathbf{u} + \mathbf{v}\|$ , is given by:

$$\|\mathbf{u} + \mathbf{v}\| = \|(1 + 3, 2 + (-12), -2 + 4)\| = \|(4, -10, 2)\| = \sqrt{4^2 + (-10)^2 + 2^2} = \sqrt{16 + 100 + 4} = \sqrt{120} = 2\sqrt{30}$$

So,  $\|\mathbf{u} + \mathbf{v}\| = 2\sqrt{30}$ .

d. The norm (magnitude) of the scalar multiple  $k\mathbf{u}$ , denoted as  $\|k\mathbf{u}\|$ , where  $k = -3$ , is given by:

$$\|k\mathbf{u}\| = \|(-3) \cdot (1, 2, -2)\| = \|(-3, -6, 6)\| = \sqrt{(-3)^2 + (-6)^2 + 6^2} = \sqrt{9 + 36 + 36} = \sqrt{81} = 9$$

So,  $\|k\mathbf{u}\| = 9$ .

6. Find  $k$  so that  $\mathbf{u}$  and  $\mathbf{v}$  are orthogonal.

a.  $\mathbf{u} = (3, k, -2)$  and  $\mathbf{v} = (6, -4, -3)$

To check for orthogonality, calculate the dot product:

$$\mathbf{u} \cdot \mathbf{v} = 3 \cdot 6 + k \cdot (-4) + (-2) \cdot (-3) = 18 - 4k + 6 = 24 - 4k$$

For the vectors to be orthogonal,  $\mathbf{u} \cdot \mathbf{v}$  must be equal to 0:

$$24 - 4k = 0$$

Solving for  $k$ :

$$4k = 24 \implies k = 6$$

b.  $\mathbf{u} = (5, k, -4, 2)$  and  $\mathbf{v} = (1, -3, 2, 2k)$

To check for orthogonality, calculate the dot product:

$$\mathbf{u} \cdot \mathbf{v} = 5 \cdot 1 + k \cdot (-3) + (-4) \cdot 2 + 2 \cdot 2k = 5 - 3k - 8 + 4k = -3k - 3$$

For the vectors to be orthogonal,  $\mathbf{u} \cdot \mathbf{v}$  must be equal to 0:

$$-3k = 3$$

Solving for  $k$ :

$$k = -1$$

c.  $\mathbf{u} = (1, 7, k+2, -2)$  and  $\mathbf{v} = (3, k, -3, k)$

To check for orthogonality, calculate the dot product:

$$\mathbf{u} \cdot \mathbf{v} = 1 \cdot 3 + 7 \cdot k + (k+2) \cdot (-3) + (-2) \cdot k = 3 + 7k - 3k - 6 - 2k$$

For the vectors to be orthogonal,  $\mathbf{u} \cdot \mathbf{v}$  must be equal to 0:

$$3 + 7k - 3k - 6 - 2k = 0$$

Solving for  $k$ :

$$-2k = 3$$

$$k = 3/(-2)$$

$$k = -\frac{3}{2}$$